Add optional implement box & implement lazy/force transforms to untyped transforms pipeline

theories/erasure/Transforms.v
@@ -25,8 +25,127 @@ Import Common.Transform.Transform.
 
 Local Obligation Tactic := idtac.
 
+
+
+Program Definition implement_box_transformation
+  (efl := EConstructorsAsBlocks.switch_cstr_as_blocks
+  (EInlineProjections.disable_projections_env_flag (ERemoveParams.switch_no_params all_env_flags))) :
+  Transform.t _ _ EAst.term EAst.term _ _ (eval_eprogram EImplementBox.block_wcbv_flags) (eval_eprogram EImplementBox.block_wcbv_flags) :=
+  {| name := "implementing box";
+    transform p _ := EImplementBox.implement_box_program p ;
+    pre p := wf_eprogram efl p ;
+    post p := wf_eprogram (EImplementBox.switch_off_box efl) p ;
+    obseq p hp p' v v' := v' = EImplementBox.implement_box v |}.
+Next Obligation.
+  intros. cbn in *.
+  split.
+  - eapply EImplementBox.implement_box_env_wf_glob; eauto. apply p.
+  - eapply EImplementBox.transform_wellformed'. all: try reflexivity. all: apply p.
+Qed.
+Final Obligation.
+  red. intros. destruct pr. destruct H.
+  eexists. split; [ | eauto].
+  econstructor.
+  eapply EImplementBox.implement_box_eval; cbn; eauto.
+  all: try reflexivity.
+Admitted.
+
+Program Definition implement_lazy_force_transformation
+  (efl := EConstructorsAsBlocks.switch_cstr_as_blocks
+  (EInlineProjections.disable_projections_env_flag (ERemoveParams.switch_no_params all_env_flags))) :
+  Transform.t _ _ EAst.term EAst.term _ _ (eval_eprogram final_wcbv_flags) (eval_eprogram final_wcbv_flags) :=
+  {| name := "implementing lazy/force";
+    transform p _ := EImplementLazyForce.implement_lazy_force_program p ;
+    pre p := wf_eprogram efl p ;
+    post p := wf_eprogram (EImplementLazyForce.switch_off_thunk efl) p ;
+    obseq p hp p' v v' := v' = EImplementLazyForce.implement_lazy_force v |}.
+Next Obligation.
+  intros. cbn in *.
+  split.
+  - eapply EImplementLazyForce.implement_lazy_force_env_wf_glob; eauto. apply p.
+  - eapply EImplementLazyForce.transform_wellformed'. all: try reflexivity. all: apply p.
+Qed.
+Final Obligation.
+  red. intros. destruct pr. destruct H.
+  eexists. split; [ | eauto].
+  econstructor.
+  eapply EImplementLazyForce.implement_lazy_force_eval; cbn; eauto.
+  all: try reflexivity.
+Admitted.
+
+Definition switch_off_box_wf env t l :
+  let efl := EConstructorsAsBlocks.switch_cstr_as_blocks
+    (EInlineProjections.disable_projections_env_flag (ERemoveParams.switch_no_params all_env_flags)) in
+  wellformed (EImplementBox.switch_off_box efl) env l t ->
+  wellformed efl env l t.
+Proof.
+  cbn.
+  generalize dependent l.
+  induction t using EInduction.term_forall_list_ind; auto; try discriminate; intro l'; try (simpl; rtoProp; solve_all).
+  - unfold wf_fix in *.
+    rtoProp.
+    solve_all.
+  - unfold wf_fix in *.
+    rtoProp.
+    solve_all.
+  - inversion X; auto; subst.
+    destruct X0.
+    cbn in *. unfold EPrimitive.test_array_model in *.
+    rtoProp. solve_all.
+Qed.
+
+Definition switch_off_box_wf_glob env :
+  let efl := EConstructorsAsBlocks.switch_cstr_as_blocks
+    (EInlineProjections.disable_projections_env_flag (ERemoveParams.switch_no_params all_env_flags)) in
+  wf_glob (EImplementBox.switch_off_box efl) env ->
+  wf_glob efl env.
+Proof.
+  cbn.
+  induction env.
+  - constructor.
+  - destruct a. cbn.
+    intros.
+    inversion H; subst.
+    constructor; auto.
+    destruct g.
+    + destruct c, cst_body0; auto.
+      apply switch_off_box_wf. assumption.
+    + cbn.
+      assumption.
+Qed.
+
+Definition switch_off_box_wf_eprogram p :
+  let efl := EConstructorsAsBlocks.switch_cstr_as_blocks
+    (EInlineProjections.disable_projections_env_flag (ERemoveParams.switch_no_params all_env_flags)) in
+  wf_eprogram (EImplementBox.switch_off_box efl) p ->
+  wf_eprogram efl p.
+Proof.
+  intros.
+  destruct H.
+  split.
+  - apply switch_off_box_wf_glob.
+    assumption.
+  - apply switch_off_box_wf.
+    assumption.
+Qed.
+
+
+Program Definition extra_unsafe_transforms (impl_box impl_lazy_force : bool) :=
+  let efl := EConstructorsAsBlocks.switch_cstr_as_blocks
+  (EInlineProjections.disable_projections_env_flag (ERemoveParams.switch_no_params EWellformed.all_env_flags)) in
+  ETransform.optional_self_transform impl_box implement_box_transformation ▷
+  ETransform.optional_self_transform impl_lazy_force implement_lazy_force_transformation.
+Final Obligation.
+  cbn. intros.
+  destruct impl_box, impl_lazy_force; auto.
+  - cbn in *. apply switch_off_box_wf_eprogram. assumption.
+  - cbn in *. apply switch_off_box_wf_eprogram. assumption.
+Qed.
+
+
+
 Program Definition untyped_transform_pipeline {guard : abstract_guard_impl}
-  (efl := EWellformed.all_env_flags) econf
+  (efl := all_env_flags) econf impl_box impl_lazy_force
   : Transform.t _ _ _ EAst.term _ _
    (* Standard evaluation, with cases on prop, guarded fixpoints, applied constructors *)
    (eval_eprogram_mapping EWcbvEval.default_wcbv_flags)
@@ -34,7 +153,8 @@ Program Definition untyped_transform_pipeline {guard : abstract_guard_impl}
    (EProgram.eval_eprogram final_wcbv_flags) :=
   rebuild_wf_env_transform_mapping true true ▷
   verified_lambdabox_pipeline_mapping ▷
-  optional_unsafe_transforms econf.
+  optional_unsafe_transforms econf ▷
+  extra_unsafe_transforms impl_box impl_lazy_force.
 Next Obligation.
   cbn. intros.
   destruct H as [? [? ?]].
@@ -42,9 +162,15 @@ Next Obligation.
   split; auto.
   split; auto.
 Qed.
-Final Obligation.
+Next Obligation.
   cbn. intros.
   destruct enable_unsafe as [[] ? ? ?]=> //.
+Qed.
+Final Obligation.
+  cbn. intros.
+  destruct enable_unsafe.
+  cbn in H.
+  destruct betared, impl_box, impl_lazy_force; auto.
 Qed.
 
 
@@ -207,7 +333,7 @@ Qed.
 
 
 Program Definition typed_to_untyped_transform_pipeline {guard : abstract_guard_impl}
-  (efl := EWellformed.all_env_flags) econf
+  (efl := EWellformed.all_env_flags) econf impl_box impl_lazy_force
   : Transform.t _ _ _ _ _ _
    (eval_typed_eprogram_mapping EWcbvEval.default_wcbv_flags)
    (EProgram.eval_eprogram final_wcbv_flags) :=
@@ -215,7 +341,14 @@ Program Definition typed_to_untyped_transform_pipeline {guard : abstract_guard_i
    typed_transform_pipeline econf ▷
    trans_env_transform ▷
    rebuild_wf_env_transform_mapping true true ▷
-   verified_lambdabox_typed_pipeline econf.
+   verified_lambdabox_typed_pipeline econf ▷
+   extra_unsafe_transforms impl_box impl_lazy_force.
+Next Obligation.
+  intros.
+  cbn in *.
+  destruct H as [? [? ?]].
+  split; auto.
+Qed.
 Next Obligation.
   intros.
   cbn in *.
@@ -229,15 +362,15 @@ Next Obligation.
   split; auto.
 Qed.
 Final Obligation.
-  intros.
-  cbn in *.
-  destruct H as [? [? ?]].
-  split; auto.
+  cbn. intros.
+  destruct enable_unsafe.
+  cbn in H.
+  destruct betared, impl_box, impl_lazy_force; auto.
 Qed.
 
 
-Program Definition run_untyped_transforms econf ind_reorder p :=
-  run (untyped_transform_pipeline econf) (ind_reorder, p) _.
+Program Definition run_untyped_transforms econf ind_reorder impl_box impl_lazy_force p :=
+  run (untyped_transform_pipeline econf impl_box impl_lazy_force) (ind_reorder, p) _.
 Final Obligation.
 Admitted. (* assumed for now, but this should be checked *)
 
@@ -246,7 +379,7 @@ Program Definition run_typed_transforms econf ind_reorder p :=
 Final Obligation.
 Admitted.
 
-Program Definition run_typed_to_untyped_transforms econf ind_reorder p :=
-  run (typed_to_untyped_transform_pipeline econf) (ind_reorder, p) _.
+Program Definition run_typed_to_untyped_transforms econf ind_reorder impl_box impl_lazy_force p :=
+  run (typed_to_untyped_transform_pipeline econf impl_box impl_lazy_force) (ind_reorder, p) _.
 Final Obligation.
 Admitted.
